Use binary ntree for trace states
Also optimize performances by adding an optional censoring domain that
determines the set of registers to hardwire to None (completely ignore
the values of these registers).

In the future we will need a better more efficient implentation of
delta_equivb...

Picinae_calling.v
@@ -63,7 +63,16 @@ Next Obligation. Proof. decide equality. Defined.
 Program Instance exp_EqDec: EqDec exp.
 Next Obligation. Proof. decide equality; apply iseq. Defined.
 
+Program Instance bool_EqDec : EqDec bool.
+Next Obligation. Proof. decide equality. Defined.
+
 Program Instance option_EqDec A `(EA : EqDec A) : EqDec (option A).
+Next Obligation. Proof. decide equality. apply iseq. Defined.
+
+Program Instance tuple_EqDec A B `(EA : EqDec A) `(EA : EqDec B): EqDec (A * B).
+Next Obligation. Proof. decide equality; apply iseq. Defined.
+
+Program Instance list_EqDec A `(EA : EqDec A) : EqDec (list A).
 Next Obligation. Proof. decide equality. apply iseq. Defined.
 
 (* Sets *)
@@ -128,6 +137,8 @@ Fixpoint set_add_all (s1: set) (l2: list N): set :=
   | nil => s1
   | h::t => set_add h (set_add_all s1 t)
   end.
+
+Definition list_to_set (l: list N): set := set_add_all set_nil l.
 
 Definition set_ap (s1 s2: set): set :=
   set_add_all s1 (set_elems s2).
@@ -316,78 +327,142 @@ Qed.
 (* We define a store delta as a variable to partial mapping onto
  * some expression. This is partial to account for "undefined" variables (which
  * could also be undefined "memory" variables) *)
-Definition store_delta := var -> option exp.
+Definition store_delta := list (var * option exp).
 
-Definition has_delta (h: hdomain) (s0 s: store) (δ: store_delta) :=
-  forall v e val (LUv: δ v = Some e) (EE: eval_exp h s0 e val), s v = val.
+(* Convert a list of variables and their values to a store function. *)
+Fixpoint updlst s (l: store_delta) : var ⇀ exp :=
+  match l with nil => s | (v,u)::t => update (updlst s t) v u end.
 
-(*
-Definition safety (c0: typctx) (se: simple_exp) :=
-  forall v0 off w (EQ_V: se = VarOff v0 off w), c0 v0 = Some (NumT w).
+(* Remove a variable from a list of variables and their values. *)
+Fixpoint remlst v (l: store_delta) : store_delta :=
+  match l with
+  | nil => nil
+  | (v',u)::t => if v == v' then remlst v t else (v',u)::(remlst v t)
+  end.
 
-Definition delta_safety (c0: typctx) (δ: store_delta) :=
-  forall v, safety c0 (δ v).
+Definition setlst (l: store_delta) v e: store_delta := (v, e) :: remlst v l.
+Notation "f [[ x := y ]]" := (setlst f x y) (at level 50, left associativity).
 
-Definition delta_models (c0 c: typctx) (δ: store_delta) :=
-  forall v t (CV: c v = Some t) (NotCpx: δ v <> Complex), hastyp_simple_exp c0 (δ v) t.
-*)
+Definition vdomain := var -> bool.
+Definition init_delta (domain: vdomain): var ⇀ exp := fun v =>
+  if domain v then Some (Var v) else None.
+Notation "f << domain >> [[ x ]]" :=
+  (updlst (init_delta domain) f x)
+  (at level 50, left associativity).
 
-Definition delta_nounk (δ: store_delta) :=
-  forall v e (LUv: δ v = Some e), forall_exps_in_exp not_unknown e.
+Definition has_delta (vd: vdomain) (h: hdomain) (s0 s: store) (δ: store_delta) :=
+  forall v e val (LUv: δ<<vd>>[[v]] = Some e) (EE: eval_exp h s0 e val), s v = val.
 
-Definition delta_differentb vars (δ1 δ2: store_delta) :=
-  existsb (fun v => if δ1 v == δ2 v then false else true) vars.
+Definition delta_nounk (vd: vdomain) (δ: store_delta) :=
+  forall v e (LUv: δ<<vd>>[[v]] = Some e), forall_exps_in_exp not_unknown e.
 
-Definition delta_different (δ1 δ2: store_delta) :=
-  exists v, δ1 v <> δ2 v.
+Definition delta_defined (δ: store_delta) :=
+  map fst δ.
 
-Definition delta_same (δ1 δ2: store_delta) :=
-  forall v, δ1 v = δ2 v.
+Definition delta_equivb (vd: vdomain) (δ1 δ2: store_delta) :=
+  forallb (fun '(v, _) => iseqb (δ1<<vd>>[[v]]) (δ2<<vd>>[[v]])) (δ1 ++ δ2).
 
-Definition delta_same_domain (δ1 δ2: store_delta) :=
-  forall v, match (δ1 v), (δ2 v) with
+Definition delta_equiv (vd: vdomain) (δ1 δ2: store_delta) :=
+  forall v, δ1<<vd>>[[v]] = δ2<<vd>>[[v]].
+
+Definition delta_same_domain (vd: vdomain) (δ1 δ2: store_delta) :=
+  forall v, match (δ1<<vd>>[[v]]), (δ2<<vd>>[[v]]) with
             | Some _, Some _ => True
             | None, None => True
             | _, _ => False
             end.
 
-Definition domain_total vars (δ: store_delta) :=
-  forall v e, δ v = Some e -> In v vars.
-
-Theorem delta_different_differentb_equiv: forall vars δ1 δ2
-  (DT1: domain_total vars δ1) (DT2: domain_total vars δ2),
-  delta_differentb vars δ1 δ2 = true <-> delta_different δ1 δ2.
+Theorem updlst_def: forall f δ v (ND: ~(In v (delta_defined δ))),
+  updlst f δ v = f v.
 Proof.
-  unfold delta_different, delta_differentb, domain_total. split.
-  - (* -> *) intro DDB. unfold delta_different. apply existsb_exists in DDB.
-    destruct DDB as [v [InDomain EQ]]. eexists. destruct iseq. discriminate.
-    eassumption.
-  - (* <- *) intro DB. apply existsb_exists. destruct DB as [v NEQ]. eexists.
-    split; [|vantisym (δ1 v) (δ2 v); [reflexivity|assumption]].
-    destruct (δ1 v) eqn: LU1; destruct (δ2 v) eqn: LU2;
-      (* When one is not empty *) try ((eapply DT1 + eapply DT2); eassumption).
-      (* Both are empty, discriminate. *) rewrite <- LU1 in NEQ.
-      contradiction (NEQ eq_refl).
+  induction δ; intros.
+  - reflexivity.
+  - simpl. destruct a as [v' e']. rewrite update_frame. apply IHδ.
+    intros Contra. apply ND. right. assumption.
+    intro. subst. apply ND. left. reflexivity.
 Qed.
 
-Corollary delta_different_differentb_equiv_contra: forall vars δ1 δ2
-  (DT1: domain_total vars δ1) (DT2: domain_total vars δ2),
-  delta_differentb vars δ1 δ2 = false <-> ~ delta_different δ1 δ2.
+Lemma neq_sym: forall A (n m: A), n <> m -> m <> n.
 Proof.
-  intros. einstantiate trivial (delta_different_differentb_equiv vars δ1 δ2) as Equiv.
-  split.
-  - intros N_DDB DB. apply Equiv in DB. rewrite N_DDB in DB. discriminate.
-  - intros N_DD. destruct delta_differentb; try reflexivity.
-    contradiction N_DD. apply Equiv. reflexivity.
+  intros. intro. subst. apply H. reflexivity.
 Qed.
 
-Theorem delta_different_same: forall δ1 δ2,
-  delta_same δ1 δ2 <-> ~ delta_different δ1 δ2.
+Theorem delta_remlst_removed: forall δ fn v,
+  updlst fn (remlst v δ) v = fn v.
+Proof.
+  intros. apply updlst_def. intros Contra. revert v Contra. induction δ; intros. 
+  - inversion Contra.
+  - simpl in Contra. destruct a as [v' u']. eapply IHδ. destruct (v == v').
+    eassumption. apply neq_sym in n. destruct Contra; [contradiction n|assumption].
+Qed.
+
+Theorem delta_remlst_frame: forall δ fn x z (NEQ: z ≠ x),
+  updlst fn (remlst x δ) z = updlst fn δ z.
+Proof.
+  induction δ; intros.
+  - reflexivity.
+  - simpl. destruct a as [v' e']. destruct (z == v').
+    + subst. apply neq_sym in NEQ. vantisym x v' by assumption. simpl.
+      repeat rewrite update_updated. reflexivity.
+    + simpl. rewrite update_frame by assumption. destruct (x == v').
+      apply IHδ. assumption. simpl. rewrite update_frame by assumption.
+      apply IHδ. assumption.
+Qed.
+
+Theorem delta_update_updated: forall fn δ x y, updlst fn (δ [[x := y]]) x = y.
+Proof. intros. unfold setlst. simpl. apply update_updated. Qed.
+
+Theorem delta_update_frame: forall δ fn x y z (NEQ: z ≠ x),
+  updlst fn (δ [[x := y]]) z = updlst fn δ z.
+Proof.
+  intros. unfold setlst. simpl. rewrite update_frame by assumption.
+  apply delta_remlst_frame. assumption.
+Qed.
+
+Theorem delta_updlst_iff_defined: forall f δ v,
+  In v (delta_defined δ) <-> In (v, updlst f δ v) δ.
 Proof.
   split.
-  - (* -> *) intro DS. intro. destruct H. apply H. apply DS.
-  - (* <- *) intros DS. intro v. destruct (δ1 v == δ2 v); try assumption.
-    destruct DS. exists v. apply n.
+  - intro InDef. revert_all. induction δ; intros.
+    + inversion InDef.
+    + simpl in *. destruct a as [v' e']. destruct (v == v').
+      * subst. left. rewrite update_updated. reflexivity.
+      * destruct InDef. subst. contradiction n. reflexivity. right.
+        rewrite update_frame by assumption. apply IHδ; assumption.
+  - intro InDelta. revert_all. induction δ; intros.
+    + inversion InDelta.
+    + destruct a as [v' e']. destruct (v == v'); subst; simpl in *.
+      * left. reflexivity.
+      * destruct InDelta. inversion H. subst. contradict n. reflexivity.
+        right. apply IHδ. rewrite update_frame in H; assumption.
+Qed.
+
+Corollary delta_updlst_iff_defined_contra: forall f δ v,
+  ~ In v (delta_defined δ) <-> ~ In (v, updlst f δ v) δ.
+Proof. intros. contrapositive delta_updlst_iff_defined. Qed.
+
+Theorem delta_equivb_iff_delta_equiv: forall vd δ1 δ2,
+  delta_equivb vd δ1 δ2 = true <-> delta_equiv vd δ1 δ2.
+Proof.
+  unfold delta_equiv, delta_equivb. split; intro EQV.
+  - (* -> *) intro. rewrite forallb_app, andb_true_iff in EQV.
+    destruct EQV as [EQV1 EQV2]. edestruct (in_dec iseq (v, δ1<<vd>>[[v]])).
+    + eapply forallb_forall in EQV1; [|eassumption]. simpl in EQV1.
+      unfold iseqb in EQV1. destruct (_ == _); try discriminate. assumption.
+    + edestruct (in_dec iseq (v, δ2<<vd>>[[v]])).
+      * eapply forallb_forall in EQV2; [|eassumption]. simpl in EQV2.
+        unfold iseqb in EQV2. destruct (_ == _); try discriminate. assumption.
+      * repeat rewrite updlst_def; try rewrite delta_updlst_iff_defined_contra;
+        trivial2.
+  - (* <- *) rewrite forallb_forall. intros. destruct x as [v e]. rewrite EQV.
+    unfold iseqb. vreflexivity (δ2<<vd>>[[v]]). reflexivity.
+Qed.
+
+Corollary delta_equivb_iff_delta_equiv_contra: forall vd δ1 δ2,
+  delta_equivb vd δ1 δ2 = false <-> ~ delta_equiv vd δ1 δ2.
+Proof.
+  intros. rewrite <- not_true_iff_false.
+  contrapositive delta_equivb_iff_delta_equiv.
 Qed.
 
 Lemma models_assign: forall c h s v e u t (MDL: models c s)
@@ -401,130 +476,125 @@ Proof.
     assumption. apply MDL in CV. assumption.
 Qed.
 
-Lemma neq_sym: forall A (n m: A), n <> m -> m <> n.
-Proof.
-  intros. intro. subst. apply H. reflexivity.
-Qed.
-
-Lemma has_delta_assign_None: forall h s s' δ v u (HD: has_delta h s s' δ),
-  has_delta h s (s' [v := u]) (δ [v := None]).
+Lemma has_delta_assign_None: forall vd h s s' δ v u (HD: has_delta vd h s s' δ),
+  has_delta vd h s (s' [v := u]) (δ [[v := None]]).
 Proof.
   unfold has_delta. intros. destruct (v == v0).
-  - subst. rewrite update_updated. rewrite update_updated in LUv. discriminate.
-  - apply neq_sym in n. rewrite update_frame in LUv by assumption.
-    rewrite update_frame in * by assumption. eapply HD; eassumption.
+  - subst. rewrite update_updated. rewrite delta_update_updated in LUv. discriminate.
+  - apply neq_sym in n. rewrite delta_update_frame in LUv by assumption.
+    rewrite update_frame by assumption. eapply HD; eassumption.
 Qed.
 
-Lemma has_delta_assign_Some: forall h s s' δ v e u (HD: has_delta h s s' δ)
+Lemma has_delta_assign_Some: forall vd h s s' δ v e u (HD: has_delta vd h s s' δ)
   (EQ: forall u' (EE: eval_exp h s e u'), u = u'),
-  has_delta h s (s' [v := u]) (δ [v := Some e]).
+  has_delta vd h s (s' [v := u]) (δ [[v := Some e]]).
 Proof.
   unfold has_delta. intros. destruct (v == v0).
-  - subst. rewrite update_updated. rewrite update_updated in LUv.
+  - subst. rewrite update_updated. rewrite delta_update_updated in LUv.
     inversion LUv; subst. apply EQ. assumption.
-  - apply neq_sym in n. rewrite update_frame in LUv by assumption.
-    rewrite update_frame in * by assumption. eapply HD; eassumption.
+  - apply neq_sym in n. rewrite delta_update_frame in LUv by assumption.
+    rewrite update_frame by assumption. eapply HD; eassumption.
 Qed.
 
-Lemma delta_nounk_assign_None: forall v δ (DNU: delta_nounk δ),
-  delta_nounk (δ [v := None]).
+Lemma delta_nounk_assign_None: forall vd v δ (DNU: delta_nounk vd δ),
+  delta_nounk vd (δ [[v := None]]).
 Proof.
   unfold delta_nounk. intros. destruct (v == v0).
-  - subst. rewrite update_updated in LUv. discriminate.
-  - apply neq_sym in n. rewrite update_frame in LUv by assumption.
+  - subst. rewrite delta_update_updated in LUv. discriminate.
+  - apply neq_sym in n. rewrite delta_update_frame in LUv by assumption.
     eapply DNU; eassumption.
 Qed.
 
-Lemma delta_nounk_assign_Some: forall v δ e (DNU: delta_nounk δ)
+Lemma delta_nounk_assign_Some: forall vd v δ e (DNU: delta_nounk vd δ)
   (NUnk: forall_exps_in_exp not_unknown e),
-  delta_nounk (δ [v := Some e]).
+  delta_nounk vd (δ [[v := Some e]]).
 Proof.
   unfold delta_nounk. intros. destruct (v == v0).
-  - subst. rewrite update_updated in LUv. inversion LUv; subst. assumption.
-  - apply neq_sym in n. rewrite update_frame in LUv by assumption.
+  - subst. rewrite delta_update_updated in LUv. inversion LUv; subst. assumption.
+  - apply neq_sym in n. rewrite delta_update_frame in LUv by assumption.
     eapply DNU; eassumption.
 Qed.
 
-Theorem delta_same_domain_refl: forall δ, delta_same_domain δ δ.
+Theorem delta_same_domain_refl: forall vd δ, delta_same_domain vd δ δ.
 Proof.
   unfold delta_same_domain. intros.
-  destruct (δ v); reflexivity.
+  destruct (δ<<vd>>[[v]]); reflexivity.
 Qed.
 
-Theorem delta_same_domain_assign: forall v δ1 δ2 o1 o2
+Theorem delta_same_domain_assign: forall vd v δ1 δ2 o1 o2
   (Sim: match o1, o2 with
         | Some _, Some _ => True
         | None, None => True
         | _, _ => False
         end)
-  (DSD: delta_same_domain δ1 δ2),
-  delta_same_domain (δ1 [v := o1]) (δ2 [v := o2]).
+  (DSD: delta_same_domain vd δ1 δ2),
+  delta_same_domain vd (δ1[[v := o1]]) (δ2[[v := o2]]).
 Proof.
   unfold delta_same_domain. intros. destruct (v == v0).
-  - subst. repeat rewrite update_updated. destruct o1, o2;
+  - subst. repeat rewrite delta_update_updated. destruct o1, o2;
     solve [reflexivity|contradiction Sim].
-  - apply neq_sym in n. repeat rewrite update_frame by assumption. apply DSD.
+  - apply neq_sym in n. repeat rewrite delta_update_frame by assumption. apply DSD.
 Qed.
 
-Fixpoint subst_valid (δ: store_delta) e: bool :=
+Fixpoint subst_valid (vd: vdomain) (δ: store_delta) e: bool :=
   match e with
   | Var v =>
-      match δ v with
+      match δ<<vd>>[[v]] with
       | Some e => true
       | None => false
       end
   | Word _ _ => true
-  | Load e1 e2 _ _ => subst_valid δ e1 && subst_valid δ e2
-  | Store e1 e2 e3 _ _ => subst_valid δ e1 && subst_valid δ e2 && subst_valid δ e3
-  | BinOp _ e1 e2 => subst_valid δ e1 && subst_valid δ e2
-  | UnOp _ e => subst_valid δ e
-  | Cast _ _ e => subst_valid δ e
+  | Load e1 e2 _ _ => subst_valid vd δ e1 && subst_valid vd δ e2
+  | Store e1 e2 e3 _ _ => subst_valid vd δ e1 && subst_valid vd δ e2 && subst_valid vd δ e3
+  | BinOp _ e1 e2 => subst_valid vd δ e1 && subst_valid vd δ e2
+  | UnOp _ e => subst_valid vd δ e
+  | Cast _ _ e => subst_valid vd δ e
   | Let v e e_in =>
-      if subst_valid δ e
-      then subst_valid (update δ v (Some (Word 0 0))) e_in
-      else subst_valid (update δ v None) e_in
+      if subst_valid vd δ e
+      then subst_valid vd (δ[[v := (Some (Word 0 0))]]) e_in
+      else subst_valid vd (δ[[v := None]]) e_in
   | Unknown _ => false
-  | Ite e1 e2 e3 => subst_valid δ e1 && subst_valid δ e2 && subst_valid δ e3
-  | Extract _ _ e => subst_valid δ e
-  | Concat e1 e2 => subst_valid δ e1 && subst_valid δ e2
+  | Ite e1 e2 e3 => subst_valid vd δ e1 && subst_valid vd δ e2 && subst_valid vd δ e3
+  | Extract _ _ e => subst_valid vd δ e
+  | Concat e1 e2 => subst_valid vd δ e1 && subst_valid vd δ e2
   end.
 
-Fixpoint subst_exp0 (δ: store_delta) e: exp :=
+Fixpoint subst_exp0 (vd: vdomain) (δ: store_delta) e: exp :=
   match e with
   | Var v =>
-      match δ v with
+      match δ<<vd>>[[v]] with
       | Some e => e
       | None => Unknown 0 (* Note we should return error in subst_err here *)
       end
   | Word _ _ => e
-  | Load e1 e2 en len => Load (subst_exp0 δ e1) (subst_exp0 δ e2) en len
-  | Store e1 e2 e3 en len => Store (subst_exp0 δ e1) (subst_exp0 δ e2)
-      (subst_exp0 δ e3) en len
-  | BinOp op e1 e2 => BinOp op (subst_exp0 δ e1) (subst_exp0 δ e2)
-  | UnOp op e => UnOp op (subst_exp0 δ e)
-  | Cast typ w' e => Cast typ w' (subst_exp0 δ e)
+  | Load e1 e2 en len => Load (subst_exp0 vd δ e1) (subst_exp0 vd δ e2) en len
+  | Store e1 e2 e3 en len => Store (subst_exp0 vd δ e1) (subst_exp0 vd δ e2)
+      (subst_exp0 vd δ e3) en len
+  | BinOp op e1 e2 => BinOp op (subst_exp0 vd δ e1) (subst_exp0 vd δ e2)
+  | UnOp op e => UnOp op (subst_exp0 vd δ e)
+  | Cast typ w' e => Cast typ w' (subst_exp0 vd δ e)
   | Let v e e_in =>
-      if subst_valid δ e
-      then subst_exp0 (update δ v (Some (subst_exp0 δ e))) e_in
-      else subst_exp0 (update δ v None) e_in
+      if subst_valid vd δ e
+      then subst_exp0 vd (δ[[v := (Some (subst_exp0 vd δ e))]]) e_in
+      else subst_exp0 vd (δ[[v := None]]) e_in
   | Unknown _ => e
-  | Ite e1 e2 e3 => Ite (subst_exp0 δ e1) (subst_exp0 δ e2) (subst_exp0 δ e3)
-  | Extract n1 n2 e => Extract n1 n2 (subst_exp0 δ e)
-  | Concat e1 e2 => Concat (subst_exp0 δ e1) (subst_exp0 δ e2)
+  | Ite e1 e2 e3 => Ite (subst_exp0 vd δ e1) (subst_exp0 vd δ e2) (subst_exp0 vd δ e3)
+  | Extract n1 n2 e => Extract n1 n2 (subst_exp0 vd δ e)
+  | Concat e1 e2 => Concat (subst_exp0 vd δ e1) (subst_exp0 vd δ e2)
   end.
 
-Definition subst_exp (δ: store_delta) e: option exp :=
-  if subst_valid δ e then Some (subst_exp0 δ e) else None.
+Definition subst_exp (vd: vdomain) (δ: store_delta) e: option exp :=
+  if subst_valid vd δ e then Some (subst_exp0 vd δ e) else None.
 
-Theorem subst_valid_any_Some: forall e δ1 δ2
-  (DSD: delta_same_domain δ1 δ2),
-  subst_valid δ1 e = subst_valid δ2 e.
+Theorem subst_valid_any_Some: forall vd e δ1 δ2
+  (DSD: delta_same_domain vd δ1 δ2),
+  subst_valid vd δ1 e = subst_valid vd δ2 e.
 Proof.
   induction e; intros; simpl; try erewrite IHe1 by eassumption;
   try erewrite IHe2 by eassumption; try erewrite IHe3 by eassumption;
   try erewrite IHe by eassumption; try reflexivity.
 
-  (* Var *) specialize (DSD v). destruct (δ1 v), (δ2 v);
+  (* Var *) specialize (DSD v). destruct (δ1<<vd>>[[v]]), (δ2<<vd>>[[v]]);
   try solve [contradiction DSD|reflexivity].
 
   (* Let *) destruct subst_valid eqn: SV1; erewrite IHe2; try reflexivity;
@@ -545,18 +615,19 @@ Local Ltac exp_destruction_nounk :=
              | n: N |- _ => destruct n
              end;
       repeat lazymatch goal with
-             | IH: forall (DNU: delta_nounk δ), _ |- _ =>
+             | IH: forall (DNU: delta_nounk _ δ), _ |- _ =>
                  einstantiate trivial IH as IH
              end
   end.
 
-Theorem subst_exp0_nounk: forall e δ (DNU: delta_nounk δ)
-  (SE: subst_valid δ e = true), forall_exps_in_exp not_unknown (subst_exp0 δ e).
+Theorem subst_exp0_nounk: forall vd e δ (DNU: delta_nounk vd δ)
+  (SE: subst_valid vd δ e = true),
+  forall_exps_in_exp not_unknown (subst_exp0 vd δ e).
 Proof.
   unfold subst_exp; induction e; intros; simpl in SE;
   try solve [exp_destruction_nounk; repeat split; assumption + reflexivity].
-  - (* Var *) destruct (δ v) eqn: LUv; inversion SE. subst. eapply DNU. simpl.
-    rewrite LUv. reflexivity.
+  - (* Var *) destruct (δ<<vd>>[[v]]) eqn: LUv; inversion SE. subst. eapply DNU.
+    simpl. rewrite LUv. reflexivity.
   - (* Let *) simpl. destruct subst_valid eqn: SV1.
     + (* e1 is valid *) apply IHe2. apply delta_nounk_assign_Some. assumption.
       apply IHe1; assumption. erewrite subst_valid_any_Some. eassumption.
@@ -565,14 +636,14 @@ Proof.
       assumption. assumption.
 Qed.
 
-Theorem subst_exp_nounk: forall e e' δ (DNU: delta_nounk δ)
-  (SE: subst_exp δ e = Some e'), forall_exps_in_exp not_unknown e'.
+Theorem subst_exp_nounk: forall vd e e' δ (DNU: delta_nounk vd δ)
+  (SE: subst_exp vd δ e = Some e'), forall_exps_in_exp not_unknown e'.
 Proof.
   unfold subst_exp. intros. destruct subst_valid eqn: SV; inversion SE.
   subst. apply subst_exp0_nounk; assumption.
 Qed.
 
-Ltac exp_destruction_correct :=
+Local Ltac exp_destruction_correct :=
   lazymatch goal with
   | δ: store_delta, e': exp |- _ =>
       lazymatch goal with
@@ -596,8 +667,8 @@ Ltac exp_destruction_correct :=
       end
   end.
 
-Theorem subst_exp_correct: forall s0 h e e' s δ v v'
-  (HD: has_delta h s0 s δ) (SE: subst_exp δ e = Some e') (EE: eval_exp h s e v)
+Theorem subst_exp_correct: forall vd s0 h e e' s δ v v'
+  (HD: has_delta vd h s0 s δ) (SE: subst_exp vd δ e = Some e') (EE: eval_exp h s e v)
   (EE': eval_exp h s0 e' v'), v = v'.
 Proof.
 
@@ -605,12 +676,12 @@ Proof.
 
   unfold subst_exp; induction e; intros; inversion EE; subst;
   simpl in SE; clear EE; try solve [exp_destruction_correct; reflexivity].
-  - (* Var *) destruct (δ v) eqn: LUv; inversion SE. subst. erewrite HD;
+  - (* Var *) destruct (δ<<vd>>[[v]]) eqn: LUv; inversion SE. subst. erewrite HD;
     solve [reflexivity|eassumption].
   - (* Let *) destruct subst_valid eqn: SV1.
     + (* e1 is valid *) erewrite subst_valid_any_Some in SE. eapply IHe2;
       [| eassumption | eassumption | eassumption]. apply has_delta_assign_Some.
-      assumption. intros. destruct (subst_valid _ e2) eqn: SV2; inversion SE.
+      assumption. intros. destruct (subst_valid _ _ e2) eqn: SV2; inversion SE.
       eapply IHe1; try eassumption. rewrite SV1. reflexivity.
       apply delta_same_domain_assign. reflexivity. apply delta_same_domain_refl.
     + (* e1 is not valid *) eapply IHe2; [| eassumption | eassumption | eassumption].
@@ -620,43 +691,7 @@ Proof.
       einstantiate trivial IHe2 as IHe2.
 Qed.
 
-(*
-Lemma delta_safety_assign: forall c0 v se δ (DS: delta_safety c0 δ)
-  (SSE: safety c0 se), delta_safety c0 (δ [v := se]).
-Proof.
-  unfold delta_safety, safety. intros.
-  destruct (v == v0).
-  - (* accessing our newly scoped variable *) subst.
-    rewrite update_updated in EQ_V. eapply SSE. eassumption.
-  - (* accessing some other variable *) apply neq_sym in n.
-    rewrite update_frame in EQ_V by assumption. eapply DS. eassumption.
-Qed.
-
-Lemma delta_models_weaken: forall c0 c c' δ (DMDL: delta_models c0 c δ)
-  (SS: c' ⊆ c), delta_models c0 c' δ.
-Proof.
-  unfold delta_models. intros.
-  apply DMDL; try apply SS; assumption.
-Qed.
-
-Lemma delta_models_assign: forall c0 c v δ se t (DMDL: delta_models c0 c δ)
-  (TSE: se = Complex \/ hastyp_simple_exp c0 se t),
-  delta_models c0 (c [v := Some t]) (δ [v := se]).
-Proof.
-  unfold delta_models. intros.
-  destruct (v == v0).
-  - subst. rewrite update_updated in *. rewrite update_updated in CV.
-    inversion CV. subst. destruct TSE; [contradiction NotCpx|].
-    inversion H; constructor; try assumption.
-  - apply neq_sym in n. rewrite update_frame in CV by assumption.
-    rewrite update_frame in * by assumption. destruct (δ _) eqn: LUv0;
-    try invalid NotCpx; rewrite <- LUv0 in *; einversion trivial DMDL;
-    rewrite LUv0; rewrite LUv0 in H1; inversion H1; subst; constructor;
-    assumption.
-Qed.
- *)
-
-Definition trace_states := (addr ⇀ store_delta).
+Definition trace_states := treeN store_delta.
 
   (*
  * list addr)%type.
@@ -733,24 +768,26 @@ Proof.
     + simpl. erewrite IHl; try eassumption. destruct (f a); reflexivity.
 Qed.
 
-Fixpoint simple_trace_stmt (δ: store_delta) (q: stmt): trace_state_res :=
+Fixpoint simple_trace_stmt (vd: vdomain) (δ: store_delta) (q: stmt):
+  trace_state_res :=
   match q with
   | Nop => Some ((δ, None) :: nil)
-  | Move v e => Some ((δ[v := subst_exp δ e], None) :: nil)
+  | Move v e => Some
+      ((if vd v then δ[[v := subst_exp vd δ e]] else remlst v δ, None) :: nil)
   | Jmp e =>
-      match subst_exp δ e with
+      match subst_exp vd δ e with
       | Some (Word n _) => Some ((δ, Some (Exit n)) :: nil)
       | _ => None
       end
   | Exn n => Some ((δ, Some (Raise n)) :: nil)
   | Seq q1 q2 =>
-      match simple_trace_stmt δ q1 with
+      match simple_trace_stmt vd δ q1 with
       | None => None
       | Some paths1 =>
           let res := map_option (fun '(δ', x) =>
             match x with
             | None =>
-                match simple_trace_stmt δ' q2 with
+                match simple_trace_stmt vd δ' q2 with
                 | None => None
                 | Some paths2 => Some paths2
                 end
@@ -762,7 +799,7 @@ Fixpoint simple_trace_stmt (δ: store_delta) (q: stmt): trace_state_res :=
           end
       end
   | If _ q1 q2 =>
-      match simple_trace_stmt δ q1, simple_trace_stmt δ q2 with
+      match simple_trace_stmt vd δ q1, simple_trace_stmt vd δ q2 with
       | None, _ | _, None => None
       | Some paths1, Some paths2 =>
           Some (paths1 ++ paths2)
@@ -770,62 +807,23 @@ Fixpoint simple_trace_stmt (δ: store_delta) (q: stmt): trace_state_res :=
   | Rep _ s => None
   end.
 
-(*
-Theorem preservation_simple_trace_stmt: forall c0 s0 q paths c c' δ
-  (MDL0: models c0 s0) (STyp: hastyp_stmt c0 c q c')
-  (DMDL: delta_models c0 c δ) (DS: delta_safety c0 δ)
-  (STS: simple_trace_stmt δ q = Some paths),
-  Forall (fun '(δ', x') => x' = None -> delta_models c0 c' δ') paths.
-Proof.
-  induction q; intros; inversion STyp; inversion STS; subst; clear STyp STS;
-  repeat constructor; intros.
-  - (* Nop *) eapply delta_models_weaken; eassumption.
-  - (* Move *) unfold delta_models. intros. destruct (v0 == v); subst.
-    + (* v0 = v *) rewrite update_updated. rewrite update_updated in NotCpx.
-      einversion trivial (eval_simple_exp_total s0). apply safety_simplify_exp.
-      assumption. einstantiate trivial (SS v). rewrite update_updated in H0.
-      inversion H0. subst. clear H0. eapply preservation_simplify_exp; eassumption.
-    + (* v0 <> v *) rewrite update_frame by assumption.
-      rewrite update_frame in NotCpx by assumption. apply DMDL.
-      erewrite <- (update_frame c) by eassumption. apply SS. assumption.
-      assumption.
-  - (* Jump *) destruct simplify_exp eqn: SE; inversion H2. subst.
-    repeat constructor. discriminate.
-  - (* Exception *) discriminate.
-  - (* Seq *) destruct simple_trace_stmt eqn: STS1; try discriminate.
-    destruct map_option eqn: MO; inversion H3. subst. rename l into paths1.
-    rename l0 into paths_res. clear H3. einstantiate trivial IHq1 as DMp1.
-    einstantiate trivial safety_simple_trace_stmt as DSp1.
-    clear STS1 IHq1. revert DMp1. induction_map paths1 maps_to paths_res; intros.
-    constructor. apply Forall_app. clear paths1 paths_res MO.
-    rename b into paths_res, al into paths1, bl into paths'. split.
-    + (* Top case *) destruct a as [δ1 [x1|]]; inversion F; subst; clear F.
-      -- repeat constructor. discriminate.
-      -- destruct (simple_trace_stmt _ q2) eqn: STS2; inversion H0. subst. clear H0.
-         inversion DMp1. inversion DSp1. subst. specialize (H1 eq_refl).
-         eapply IHq2; try eassumption. eapply hastyp_stmt_weaken; try eassumption.
-    + (* Inductive case *) inversion DSp1. inversion DMp1. subst.
-      eapply IHab; eassumption.
-  - (* If *) destruct simple_trace_stmt eqn: STS1; try discriminate.
-    destruct (simple_trace_stmt _ q2) eqn: STS2; try discriminate. inversion H4.
-    subst. apply Forall_app. eapply hastyp_stmt_weaken in TS1; try eassumption.
-    eapply hastyp_stmt_weaken in TS2; try eassumption. split;
-      (eapply IHq1 + eapply IHq2); eassumption.
-Qed.
-*)
-
-Theorem simple_trace_stmt_correct: forall s0 q paths h s s' x δ
-  (HD: has_delta h s0 s δ) (XS: exec_stmt h s q s' x)
-  (STS: simple_trace_stmt δ q = Some paths),
-  Exists (fun '(δ', x') => x' = x /\ has_delta h s0 s' δ') paths.
+Theorem simple_trace_stmt_correct: forall vd s0 q paths h s s' x δ
+  (HD: has_delta vd h s0 s δ) (XS: exec_stmt h s q s' x)
+  (STS: simple_trace_stmt vd δ q = Some paths),
+  Exists (fun '(δ', x') => x' = x /\ has_delta vd h s0 s' δ') paths.
 Proof.
   induction q; intros; inversion XS; inversion STS; subst; clear XS STS.
   - (* Nop *) constructor. split. reflexivity. assumption.
-  - (* Move *) constructor. split. reflexivity. destruct subst_exp eqn: SE1.
-    + apply has_delta_assign_Some. assumption. intros.
+  - (* Move *) constructor. split. reflexivity. destruct vd eqn: VD.
+    + destruct subst_exp eqn: SE1; [|apply has_delta_assign_None; assumption]. 
+      apply has_delta_assign_Some. assumption. intros.
       eapply subst_exp_correct; eassumption.
-    + apply has_delta_assign_None. assumption.
-  - (* Jmp *) destruct (subst_exp _ _) eqn: SE; try destruct e0; inversion H3.
+    + unfold has_delta. intros. destruct (v0 == v).
+      * subst. unfold init_delta in LUv. rewrite delta_remlst_removed, VD in LUv.
+        discriminate.
+      * rewrite update_frame by assumption. rewrite delta_remlst_frame in LUv by assumption.
+        eapply HD; eassumption.
+  - (* Jmp *) destruct (subst_exp _ _ _) eqn: SE; try destruct e0; inversion H3.
     subst. constructor. split; try assumption.
     einstantiate trivial subst_exp_correct as Res. constructor. inversion Res.
     reflexivity.
@@ -833,18 +831,18 @@ Proof.
   - (* Seq, exit 1 *) destruct simple_trace_stmt as [paths1|] eqn: SQ1; try discriminate.
     einstantiate trivial (IHq1). destruct map_option eqn: Map; inversion H4.
     subst. clear H4. rename l into paths_res. apply Exists_exists in H.
-    destruct H as [[δ1 x1] [InP1 [X HD1]]]; subst. apply Exists_exists.
+    destruct H as [ [δ1 x1] [InP1 [X HD1] ] ]; subst. apply Exists_exists.
     exists (δ1, Some x0). repeat split; [|assumption]. apply in_concat. eexists.
     split; [|apply in_eq]. eapply map_option_includes; try eassumption.
     reflexivity.
   - (* Seq, exit 2 *) destruct (simple_trace_stmt) eqn:SQ1; [|discriminate].
     destruct map_option eqn:MO; inversion H4. subst. clear H4. einstantiate
     trivial IHq1. apply Exists_exists in H. apply Exists_exists.
-    destruct H as [[δ1 x1] [InP1 [X HD1]]]. subst.
-    destruct (simple_trace_stmt δ1 q2) eqn:SQ2.
+    destruct H as [ [δ1 x1] [InP1 [X HD1] ] ]. subst.
+    destruct (simple_trace_stmt vd δ1 q2) eqn:SQ2.
     + einstantiate IHq2 as IHq2; try assumption; try apply SQ2; try apply TS2;
       try apply XS0; try eassumption. apply Exists_exists in IHq2.
-      destruct IHq2 as [[δ' x'] [Inl1 HD']]. eexists. split.
+      destruct IHq2 as [ [δ' x'] [Inl1 HD'] ]. eexists. split.
 
       (* Prove that state is in concat l0 *) apply in_concat. eexists.
       split; try eassumption. eapply map_option_includes; try eassumption.
@@ -853,20 +851,26 @@ Proof.
       simpl. rewrite SQ2. reflexivity.
   - (* If/else *) destruct c;
     (destruct (simple_trace_stmt) eqn: ST1; [|discriminate]);
-    (destruct (simple_trace_stmt δ q2) eqn: ST2; [|discriminate]).
+    (destruct (simple_trace_stmt vd δ q2) eqn: ST2; [|discriminate]).
     + (* q2 *) einstantiate trivial IHq2. eapply incl_Exists.
       inversion H5. apply incl_appr. apply incl_refl. assumption.
     + (* q1 *) einstantiate trivial IHq1. eapply incl_Exists.
       inversion H5. apply incl_appl. apply incl_refl. assumption.
 Qed.
 
-Definition join_states_if_changed (vars: list var) (δ1: option store_delta)
+Definition join_states_if_changed (vd: vdomain) (δ1: option store_delta)
   (δ2: store_delta): option store_delta :=
   match δ1 with
   | Some δ1 =>
-      if delta_differentb vars δ1 δ2
-      then Some (fun v => if δ1 v == δ2 v then δ2 v else None)
-      else None
+      if delta_equivb vd δ1 δ2
+      then None
+      else let δ_merge := (fold_right (fun v δ' =>
+        δ'[[v := if δ1<<vd>>[[v]] == δ2<<vd>>[[v]] then δ2<<vd>>[[v]] else None]])
+        nil (delta_defined (δ1 ++ δ2))) in
+        if delta_equivb vd δ1 δ_merge then
+            None
+        else
+            Some δ_merge 
   | None => Some δ2
   end.
 
@@ -884,7 +888,7 @@ Definition true_hyp {V} hyps (v:V) :=
   | None => True
   end.
 
-Definition process_state (vars: list var) (exitof: option exit -> exit)
+Definition process_state (vd: vdomain) (exitof: option exit -> exit)
   (st: store_delta * option exit) (accum: trace_states * bool) :=
   let '(ts, changed) := accum in
   let '(δ', x) := st in
@@ -897,8 +901,8 @@ Definition process_state (vars: list var) (exitof: option exit -> exit)
   | Exit next_addr =>
       (* Check if joining states changed something. If so, we update and mark
        * this as changed *)
-      match join_states_if_changed vars (ts next_addr) δ' with
-      | Some δ_merge => (update ts next_addr (Some δ_merge), true)
+      match join_states_if_changed vd (tget_n ts next_addr) δ' with
+      | Some δ_merge => (tupdate_n ts next_addr δ_merge, true)
       | None => (ts, changed)
       end
   | Raise _ => (ts, changed)
@@ -942,18 +946,18 @@ Proof.
   apply SS. assumption.
 Qed.
 
-Definition stmt_correct q δ x := forall s0 h s s' (XS: exec_stmt h s q s' x),
-  has_delta h s0 s' δ.
+Definition stmt_correct vd q δ x := forall s0 h s s' (XS: exec_stmt h s q s' x),
+  has_delta vd h s0 s' δ.
 
-Definition correctness_sub_prog p domain ts h a0 s0 :=
+Definition correctness_sub_prog vd p domain ts h a0 s0 :=
   (forall a1 s1 n1 δ
     (XP: exec_prog h (sub_prog p domain) a0 s0 n1 s1 (Exit a1))
-    (TS2: ts a1 = Some δ), has_delta h s0 s1 δ).
+    (TS2: tget_n ts a1 = Some δ), has_delta vd h s0 s1 δ).
 
 Inductive subgoals: Set :=
   .
 
-Definition trace_program_step_at (vars: list var) (p: program)
+Definition trace_program_step_at (vd: vdomain) (p: program)
   (hints: program -> addr -> trace_states -> option (trace_states * bool))
   addr (accum: option (trace_states * bool)) :=
   match accum with
@@ -970,13 +974,13 @@ Definition trace_program_step_at (vars: list var) (p: program)
           | None => None (*Some (ts, working, P)*)
           | Some (sz, q) =>
               (* Sanity check for if we have already visited this address *)
-              match ts addr with
+              match tget_n ts addr with
               | None => Some (ts, changed)
               | Some δ_a =>
-                  match simple_trace_stmt δ_a q with
+                  match simple_trace_stmt vd δ_a q with
                   | None => None
                   | Some next_states =>
-                      let res := fold_right (process_state vars
+                      let res := fold_right (process_state vd
                         (exitof (addr + sz))) (ts, changed) next_states in
                       Some res
                   end
@@ -986,30 +990,30 @@ Definition trace_program_step_at (vars: list var) (p: program)
       end
   end.
 
-Definition expand_trace_program (vars: list var) (p: program)
+Definition expand_trace_program (vd: vdomain) (p: program) 
   (hints: program -> addr -> trace_states -> option (trace_states * bool))
   (reachable: set) (init_ts: trace_states): option (trace_states * bool) :=
-  fold_right (trace_program_step_at vars p hints) (Some (init_ts, false))
+  fold_right (trace_program_step_at vd p hints) (Some (init_ts, false))
     (set_elems reachable).
 
 Definition iterM (n: N) {A} (f: A -> option A) (x: A) :=
   N.iter n (fun x => match x with Some x => f x | None => None end) (Some x).
 
-Definition expand_trace_program_n (n: N)
+Definition expand_trace_program_n (n: N) (vd: vdomain)
   (hints: program -> addr -> trace_states -> option (trace_states * bool))
-  (vars: list var) (p: program) (reachable: set) (init_ts: trace_states):
+  (p: program) (reachable: set) (init_ts: trace_states):
   option (trace_states * bool) :=
   N.iter n (fun x =>
     match x with
-    | Some (ts, true) => expand_trace_program vars p hints reachable ts
+    | Some (ts, true) => expand_trace_program vd p hints reachable ts
     | Some (ts, false) => Some (ts, false)
     | None => None
     end) (Some (init_ts, true)).
 
-Lemma fold_expand_trace_program: forall vars p hints reachable init_ts,
-  fold_right (trace_program_step_at vars p hints) (Some (init_ts, false))
+Lemma fold_expand_trace_program: forall vd p hints reachable init_ts,
+  fold_right (trace_program_step_at vd p hints) (Some (init_ts, false))
     (set_elems reachable) =
-  expand_trace_program vars p hints reachable init_ts.
+  expand_trace_program vd p hints reachable init_ts.
 Proof. reflexivity. Qed.
 
 Inductive exec_prog2 (h: hdomain) (p:program) (a:addr) (s:store): nat -> store -> exit -> Prop :=
@@ -1033,7 +1037,7 @@ Proof.
       * (* n = 1 *) inversion XP0. subst. rewrite <- EX. econstructor;
         try eassumption. constructor.
       * rewrite <- Nat.add_1_r in XP0. einstantiate trivial exec_prog_split as XPS.
-        destruct XPS as [s1 [a1 [XP_middle XP_end]]]. inversion XP_end. subst.
+        destruct XPS as [s1 [a1 [XP_middle XP_end] ] ]. inversion XP_end. subst.
         inversion XP1. subst. rewrite <- EX0. econstructor; try eassumption.
         apply IHn. rewrite <- Nat.add_1_l. eapply exec_prog_concat;
         [|apply XP_middle]. econstructor; try eassumption. econstructor.
@@ -1054,28 +1058,28 @@ Proof.
            destruct e; inversion EX. subst. assumption.
 Qed.
 
-Theorem trace_program_step_at_steady_correct: forall p vars a_new al hints ts
-  h a0 s0 (Init: forall δ s, ts a0 = Some δ -> has_delta h s s δ)
-  (IHal: correctness_sub_prog p al ts h a0 s0) (UNIQ: NoDup (a_new :: al))
-  (Total: Forall (fun a1 => exists δ1, ts a1 = Some δ1) (a_new :: al))
-  (TPSA: trace_program_step_at vars p hints a_new (Some (ts, false)) =
+Theorem trace_program_step_at_steady_correct: forall vd p a_new al hints ts
+  h a0 s0 (Init: forall δ s, tget_n ts a0 = Some δ -> has_delta vd h s s δ)
+  (IHal: correctness_sub_prog vd p al ts h a0 s0) (UNIQ: NoDup (a_new :: al))
+  (Total: Forall (fun a1 => exists δ1, tget_n ts a1 = Some δ1) (a_new :: al))
+  (TPSA: trace_program_step_at vd p hints a_new (Some (ts, false)) =
     Some (ts, false))
   (HintsCorrect: forall a_new al ts h a0 s0
-    (IHal: correctness_sub_prog p al ts h a0 s0) (UNIQ: NoDup (a_new :: al))
-    (Total: Forall (fun a1 => exists δ1, ts a1 = Some δ1) (a_new :: al))
+    (IHal: correctness_sub_prog vd p al ts h a0 s0) (UNIQ: NoDup (a_new :: al))
+    (Total: Forall (fun a1 => exists δ1, tget_n ts a1 = Some δ1) (a_new :: al))
     (Hint: hints p a_new ts = Some (ts, false)),
-    correctness_sub_prog p (a_new :: al) ts h a0 s0),
-  correctness_sub_prog p (a_new :: al) ts h a0 s0.
+    correctness_sub_prog vd p (a_new :: al) ts h a0 s0),
+  correctness_sub_prog vd p (a_new :: al) ts h a0 s0.
 Proof.
   (* Destruct trace_program_step_at function. *)
   unfold correctness_sub_prog. intros. simpl in TPSA.
 
   (* Using hint if available *)
-  destruct hints as [[ts' changed']|] eqn: Hint. inversion TPSA. subst.
+  destruct hints as [ [ts' changed']|] eqn: Hint. inversion TPSA. subst.
   eapply HintsCorrect; try eassumption. clear HintsCorrect.
 
-  destruct (p _ _) as [[sz_new q_new]|] eqn: LUa_new; try discriminate.
-  destruct (ts a_new) as [δ_a_new|] eqn: TSa_new; try discriminate.
+  destruct (p _ _) as [ [sz_new q_new]|] eqn: LUa_new; try discriminate.
+  destruct (tget_n ts a_new) as [δ_a_new|] eqn: TSa_new; try discriminate.
   destruct simple_trace_stmt as [next_states|] eqn: Fn; try discriminate.
   rename a1 into a', s1 into s', n1 into n', δ into δ', XP into XP',
     TS2 into TS'.
@@ -1098,7 +1102,7 @@ Proof.
     (* Prove that a1 is in the domain. Holds true because a1 was in the
      * sub-program because of our execution flow, so must be in subdomain. *)
     unfold sub_prog in LU. destruct existsb eqn: EXa2; try discriminate.
-    apply existsb_exists in EXa2. destruct EXa2 as [a1' [InDomain Eq]].
+    apply existsb_exists in EXa2. destruct EXa2 as [a1' [InDomain Eq] ].
     destruct (a1 == a1'); try discriminate. subst. assumption.
 Admitted.
 
@@ -1241,33 +1245,33 @@ Proof.
   - (* Jmp *) inversion E; subst; clear E; try discriminate; simpl in *.
     inversion JMPS. eapply set_has_in. apply set_add_correct.
   - (* Exn *) reflexivity.
-  - (* Seq, exit in q1 *) destruct (stmt_reachable q1) as [[j1 falls1]|] eqn: J1;
+  - (* Seq, exit in q1 *) destruct (stmt_reachable q1) as [ [j1 falls1]|] eqn: J1;
     try solve [destruct (stmt_reachable q2) eqn: J2; discriminate]. destruct falls1.
     + (* Can fall-through *) destruct x0; try reflexivity.
-      destruct (stmt_reachable q2) as [[j2 falls2]|] eqn: J2; try discriminate.
+      destruct (stmt_reachable q2) as [ [j2 falls2]|] eqn: J2; try discriminate.
       inversion JMPS. subst. apply set_ap_has_l. einstantiate trivial IHq1.
     + (* Cannot fall-through *) inversion JMPS. subst. destruct x0;
       try reflexivity. einstantiate trivial IHq1.
-  - (* Seq, exit in q2 *) destruct (stmt_reachable q1) as [[j1 falls1]|] eqn: J1;
+  - (* Seq, exit in q2 *) destruct (stmt_reachable q1) as [ [j1 falls1]|] eqn: J1;
     try solve [destruct (stmt_reachable q2) eqn: J2; discriminate]. destruct falls1.
-    + (* Can fall-through *) destruct (stmt_reachable q2) as [[j2 falls2]|] eqn: J2;
+    + (* Can fall-through *) destruct (stmt_reachable q2) as [ [j2 falls2]|] eqn: J2;
       try discriminate. inversion JMPS. subst. einstantiate trivial IHq2 as IHq2.
-      destruct x as [[a|n]|]; trivial2. apply set_ap_has_r. assumption.
+      destruct x as [ [a|n]|]; trivial2. apply set_ap_has_r. assumption.
     + (* Cannot fall-through; contradiction *) inversion JMPS.
       subst. einstantiate trivial IHq1 as IHq1.
-  - (* If *) destruct (stmt_reachable q1) as [[j1 falls1]|] eqn: J1;
-    destruct (stmt_reachable q2) as [[j2 falls2]|] eqn: J2; try discriminate.
-    inversion JMPS. subst. clear JMPS. destruct x as [[a|n]|]; try reflexivity.
+  - (* If *) destruct (stmt_reachable q1) as [ [j1 falls1]|] eqn: J1;
+    destruct (stmt_reachable q2) as [ [j2 falls2]|] eqn: J2; try discriminate.
+    inversion JMPS. subst. clear JMPS. destruct x as [ [a|n]|]; try reflexivity.
     + (* Jumped *) rewrite set_ap_has_split. apply orb_true_intro.
       destruct c; [einstantiate trivial IHq2; right|
         einstantiate trivial IHq1; left]; eassumption.
     + (* Fallthrough *) apply orb_true_intro. destruct c;
       [einstantiate trivial IHq2; right | einstantiate trivial IHq1; left];
       assumption.
-  - (* Evil rep *) destruct stmt_reachable as [[jmps' falls']|] eqn: Jinner;
-    inversion JMPS. subst. destruct x as [[a|?]|]; try reflexivity.
+  - (* Evil rep *) destruct stmt_reachable as [ [jmps' falls']|] eqn: Jinner;
+    inversion JMPS. subst. destruct x as [ [a|?]|]; try reflexivity.
     einstantiate trivial rep_exits_total as RET.
-    destruct RET as [s2 [s2' XSinner]]. einstantiate trivial IHq.
+    destruct RET as [s2 [s2' XSinner] ]. einstantiate trivial IHq.
 Qed.
 
 Lemma reachables_incl: forall hints p a reaches' reaches
@@ -1276,8 +1280,8 @@ Lemma reachables_incl: forall hints p a reaches' reaches
 Proof.
   unfold reachables_at. intros. destruct hints eqn: Hints.
   - inversion RA. subst. intros a2 InS. apply set_ap_right. assumption.
-  - destruct p as [[sz q]|] eqn: LU; try discriminate.
-    destruct stmt_reachable as [[jmps falls]|] eqn: SRQ; try discriminate.
+  - destruct p as [ [sz q]|] eqn: LU; try discriminate.
+    destruct stmt_reachable as [ [jmps falls]|] eqn: SRQ; try discriminate.
     inversion RA. subst. intros a2 InS. apply set_ap_right. assumption.
 Qed.
 
@@ -1307,8 +1311,8 @@ Lemma destruct_reachables_at_prin: forall {P hints p a_new reaches reaches'}
 Proof.
   intros. simpl in RA.
   destruct hints eqn: Hints. inversion RA. subst. eapply PHints; reflexivity.
-  destruct p as [[sz q]|] eqn: LU; try discriminate.
-  destruct stmt_reachable as [[sjmps falls]|] eqn: SR; inversion RA. subst.
+  destruct p as [ [sz q]|] eqn: LU; try discriminate.
+  destruct stmt_reachable as [ [sjmps falls]|] eqn: SR; inversion RA. subst.
   eapply PDefault; solve [reflexivity|eassumption].
 Qed.
 
@@ -1352,7 +1356,7 @@ Proof.
       * (* Provided by our info *) erewrite sub_prog_nwc_pres in LU0 by assumption.
         erewrite sub_prog_SS in LU by eassumption. inversion LU. subst.
         einstantiate trivial stmt_reachable_complete. apply set_has_in.
-        rewrite <- RA'. destruct x' as [[a|?]|]; try inversion EX; subst.
+        rewrite <- RA'. destruct x' as [ [a|?]|]; try inversion EX; subst.
         -- (* Some exit *) apply set_has_in in H. apply set_ap_left.
            destruct falls; [apply set_add_preserves|]; assumption.
         -- (* fallthru *) apply set_ap_left. apply set_add_correct.
@@ -1412,7 +1416,7 @@ Proof.
   unfold expand_reachables_n, iterM. intros. revert ER XP.
   remember (fun _ => _) as fn. pattern (N.iter iter fn (Some (reaches, true))).
   apply N.iter_invariant; try discriminate. intros. subst.
-  destruct x as [[r fin]|]; try discriminate.
+  destruct x as [ [r fin]|]; try discriminate.
   destruct fin; [|inversion ER; subst; apply H; trivial2].
   erewrite (expand_reachables_equiv_equal r) in ER by eassumption.
   eapply expand_reachables_complete_inv; try eassumption.
@@ -1480,7 +1484,7 @@ Theorem welltyped_prog_sub: forall p a c (WT: welltyped_prog c p),
   welltyped_prog c (sub_prog p a).
 Proof.
   intros. unfold welltyped_prog. intros.
-  destruct sub_prog as [[sz q]|] eqn: SUB; try reflexivity.
+  destruct sub_prog as [ [sz q]|] eqn: SUB; try reflexivity.
   specialize (WT s a0) as WT. unfold sub_prog in SUB.
   destruct existsb; try discriminate. rewrite SUB in WT. assumption.
 Qed.
@@ -1490,83 +1494,7 @@ Require Import strchr_i386.
 Require Import test.
 Import X86Notations.
 
-Definition compactify_delta (δ: store_delta): store_delta :=
-  fun (v: var) =>
-    match v with
-    | V_MEM32 => δ V_MEM32
-    (* Flags (1-bit registers): *)
-    | R_AF => δ R_AF
-    | R_CF => δ R_CF
-    | R_DF => δ R_DF
-    | R_OF => δ R_OF
-    | R_PF => δ R_PF
-    | R_SF => δ R_SF
-    | R_ZF => δ R_ZF
-    (* Segment selectors (16-bit registers): *)
-    | R_CS => δ R_CS
-    | R_DS => δ R_DS
-    | R_ES => δ R_ES
-    | R_FS => δ R_FS
-    | R_GS => δ R_GS
-    | R_SS => δ R_SS
-    (* Floating point control register (16-bit): *)
-    | R_FPU_CONTROL => δ R_FPU_CONTROL (* NumT 16 *)
-    (* Floating point registers (80-bit): *)
-    | R_ST0 => δ R_ST0
-    | R_ST1 => δ R_ST1
-    | R_ST2 => δ R_ST2
-    | R_ST3 => δ R_ST3
-    | R_ST4 => δ R_ST4
-    | R_ST5 => δ R_ST5
-    | R_ST6 => δ R_ST6
-    | R_ST7 => δ R_ST7 (* NumT 80 *)
-    (* General-purpose registers (32-bit): *)
-    | R_EAX => δ R_EAX
-    | R_EBX => δ R_EBX
-    | R_ECX => δ R_ECX
-    | R_EDX => δ R_EDX
-    | R_EDI => δ R_EDI
-    | R_ESI => δ R_ESI
-    (* Stack pointer and base pointer (32-bit): *)
-    | R_ESP => δ R_ESP
-    | R_EBP => δ R_EBP
-    (* Modifiable segment base registers (32-bit): *)
-    | R_FS_BASE => δ R_FS_BASE
-    | R_GS_BASE => δ R_GS_BASE
-    (* Descriptor table registers (32-bit): *)
-    | R_LDTR => δ R_LDTR
-    | R_GDTR => δ R_GDTR
-    (* SSE control register (32-bit): *)
-    | R_MXCSR => δ R_MXCSR (* NumT 32 *)
-    (* MMX and SSE registers (256-bit): *)
-    | R_YMM0 => δ R_YMM0
-    | R_YMM1 => δ R_YMM1
-    | R_YMM2 => δ R_YMM2
-    | R_YMM3 => δ R_YMM3
-    | R_YMM4 => δ R_YMM4
-    | R_YMM5 => δ R_YMM5
-    | R_YMM6 => δ R_YMM6
-    | R_YMM7 => δ R_YMM7
-    | R_YMM8 => δ R_YMM8
-    | R_YMM9 => δ R_YMM9
-    | R_YMM10 => δ R_YMM10
-    | R_YMM11 => δ R_YMM11
-    | R_YMM12 => δ R_YMM12
-    | R_YMM13 => δ R_YMM13
-    | R_YMM14 => δ R_YMM14
-    | R_YMM15 => δ R_YMM15
-    (* These meta-variables model page access permissions: *)
-    | A_READ => δ A_READ
-    | A_WRITE => δ A_WRITE
-    | V_TEMP n => δ (V_TEMP n)
-    end.
-
 Definition fh := htotal.
-
-Definition init_store_delta: store_delta :=
-  fun v => Some (Var v).
-
-Definition vars := R_EBP :: R_ESP :: nil.
 
 Definition simp_prog: program := fun _ a =>
   match a with
@@ -1587,16 +1515,16 @@ Qed.
 Definition simp_prog_trace_hint (p: program) (a: addr) (ts: trace_states):
   option (trace_states * bool) := None.
 
-Definition simp_prog_trace reachables := expand_trace_program_n 10
-  simp_prog_trace_hint vars simp_prog reachables (update ⊥ 0 (Some init_store_delta)).
+Definition simp_prog_trace reachables := expand_trace_program_n 10 (fun _ => true)
+  simp_prog_trace_hint simp_prog reachables (tupdate_n treeN_nil 0 nil).
 
 Goal True.
 Proof.
 
   pose (x := match simp_prog_trace {{0;1}} with
              | Some (ts, b) =>
-                 match ts 1 with
-                 | Some δ => Some (compactify_delta δ, b)
+                 match tget_n ts 1 with
+                 | Some δ => Some (ts, δ, b)
                  | None => None
                  end
              | None => None
@@ -1611,9 +1539,9 @@ Proof.
   Picinae_typecheck.
 Qed.
 
-Definition my_prog_reachables_hint (ret: addr) (a: addr): option (set addr) :=
+Definition my_prog_reachables_hint (ret: addr) (a: addr): option set :=
   match a with
-  | 34 => Some (ret::nil)
+  | 34 => Some {{ret}}
   | _ => None
   end.
 
@@ -1627,26 +1555,27 @@ Definition my_prog_trace_hint (p: program) (a: addr) (ts: trace_states):
   | _ => None
   end.
 
-Definition my_prog_trace reachables := expand_trace_program_n 10
-  my_prog_trace_hint vars my_prog reachables (update ⊥ 0 (Some init_store_delta)).
+Definition my_prog_trace x reachables := expand_trace_program_n x (fun _ => true)
+  my_prog_trace_hint my_prog reachables (tupdate_n treeN_nil 0 nil).
+
+Ltac unbox_res v :=
+  match eval red in v with
+  | Some (?v', _) => clear v; pose (v := v')
+  end.
+
+Ltac unbox_Some v :=
+  match eval red in v with
+  | Some ?v' => clear v; pose (v := v')
+  end.
+
 
 Goal True.
 Proof.
 
-  pose (x := my_prog_reachables 0).
-  compute in x.
-  match eval compute in x with
-  | Some (?v, nil) => clear x; pose (reachables := v)
-  end.
-  pose (x := match my_prog_trace reachables with
-             | Some (ts, b) =>
-                 match ts 34 with
-                 | Some δ => Some (compactify_delta δ, b)
-                 | None => None
-                 end
-             | None => None
-             end).
-  compute in x.
+  pose (reachables := my_prog_reachables 0).
+  compute in reachables. unbox_res reachables.
+  pose (x := my_prog_trace 100 (list_to_set reachables)). compute in x.
+
 Abort.
 
 Definition ret_pres (esp0:N) (mem:addr->N) (s:store) :=
@@ -1666,11 +1595,9 @@ Proof.
   Picinae_typecheck.
 Qed.
 
-
-
-Definition strchr_reachables_hint (ret: addr) (a: addr): option (set addr) :=
+Definition strchr_reachables_hint (ret: addr) (a: addr): option set :=
   match a with
-  | 401 => Some (ret::nil)
+  | 401 => Some {{ret}}
   | _ => None
   end.
 
@@ -1684,8 +1611,30 @@ Definition strchr_trace_hint (p: program) (a: addr) (ts: trace_states):
   | _ => None
   end.
 
-Definition strchr_trace reachables := expand_trace_program_n 1
-  strchr_trace_hint vars strchr_i386 reachables (update ⊥ 0 (Some init_store_delta)).
+Require Extraction.
+Extraction Language OCaml.
+
+Definition domain1 var :=
+  match var with
+  | V_TEMP _ => false
+  | R_AF | R_CF | R_DF | R_OF | R_PF | R_SF | R_ZF => false
+  | R_EAX | R_ECX | R_EDX => false
+  | _ => true
+  end.
+
+Definition strchr_trace reachables := expand_trace_program_n 100 (fun _ => true)
+  strchr_trace_hint strchr_i386 reachables (tupdate_n treeN_nil 0 nil).
+
+Definition strchr_trace2 reachables := expand_trace_program_n 100 domain1
+  strchr_trace_hint strchr_i386 reachables (tupdate_n treeN_nil 0 nil).
+
+Extract Inductive bool => "bool" [ "true" "false" ].
+Extract Inductive option => "option" [ "Some" "None" ].
+Extract Inductive prod => "( * )"  [ "(,)" ].
+Extract Inductive list => "list" [ "[]" "(::)" ].
+Require Import ExtrOcamlIntConv.
+Extraction "calling" strchr_trace strchr_trace2 strchr_reachables list_to_set
+  n_of_int int_of_n.
 
 Goal True.
 Proof.
@@ -1696,6 +1645,9 @@ Proof.
   match eval compute in x with
   | Some (?v, nil) => clear x; pose (reachables := v)
   end.
+  pose (x := strchr_trace2 (list_to_set reachables)).
+  time (vm_compute in x).
+
   pose (x := match strchr_trace reachables with
              | Some (ts, b) =>
                  match ts 401 with
